\documentclass{article}
\usepackage{amsmath}
\begin{document}


\\Task - Normalization


((\lambda a.(\lambda b.b\ b)\ (\lambda b.b\ b))\ b)\ ((\lambda c.(c\ b))\ (\lambda a.a)) \rightarrow_\beta$$

((\lambda b.b\ b)\ (\lambda b.b\ b))\ ((\lambda c.(c\ b))\ (\lambda a.a)) \rightarrow_\beta$$

((\lambda b.b\ b)\ (\lambda b.b\ b))\ ((\lambda a.a)\ b) \rightarrow_\beta$$

((\lambda b.b\ b)\ (\lambda b.b\ b))\ b \rightarrow_\beta$$


\\Task - S K K

((\lambda x y z.x z (y z)) (\lambda x y.x) (\lambda x y.x)) \rightarrow_\beta$$

((\lambda y z.(\lambda x y.x) z (y z)) (\lambda x y.x)) \rightarrow_\beta$$

((\lambda z. (\lambda x y.x) z ((\lambda x y.x)z))) \rightarrow_\beta$$

((\lambda z. (\lambda y.z) ((\lambda x y.x)z))) \rightarrow_\beta$$

((\lambda z. (\lambda ((\lambda x y.x)z).z) ))\rightarrow_\beta$$ 
((\lambda z. z)) = I
    
\end{document}
